theories/lifetime/na_borrow.v
@@ -14,14 +14,19 @@ Section na_bor.
   Context `{invG Σ, lftG Σ, na_invG Σ}
           (tid : na_inv_pool_name) (N : namespace) (P : iProp Σ).
 
-  Global Instance na_bor_ne κ tid N n :
-    Proper (dist n ==> dist n) (na_bor κ tid N).
+  Global Instance na_bor_ne κ n : Proper (dist n ==> dist n) (na_bor κ tid N).
   Proof. solve_proper. Qed.
-  Global Instance na_bor_contractive κ tid N : Contractive (na_bor κ tid N).
+  Global Instance na_bor_contractive κ : Contractive (na_bor κ tid N).
   Proof. solve_contractive. Qed.
-  Global Instance na_bor_proper κ tid N :
-    Proper ((⊣⊢) ==> (⊣⊢)) (na_bor κ tid N).
+  Global Instance na_bor_proper κ : Proper ((⊣⊢) ==> (⊣⊢)) (na_bor κ tid N).
   Proof. solve_proper. Qed.
+  Lemma na_bor_iff_proper κ P' :
+    ▷ □ (P ↔ P') -∗ &na{κ, tid, N} P -∗ &na{κ, tid, N} P'.
+  Proof.
+    iIntros "HPP' H". iDestruct "H" as (i) "[HP ?]". iExists i. iFrame.
+    iApply (idx_bor_iff_proper with "HPP' HP").
+  Qed.
+
   Global Instance na_bor_persistent κ : PersistentP (&na{κ,tid,N} P) := _.
 
   Lemma bor_na κ E : ↑lftN ⊆ E → &{κ}P ={E}=∗ &na{κ,tid,N}P.
